theories/examples/susp_correctness/definitions.v
@@ -421,14 +421,14 @@ Section authenticatable_definitions.
   Definition suspend_v_deser_spec
       (suspend v_deser : val) (A : lrel_tern Σ) (t : evi_type) : iProp Σ :=
     □(∀ t' (a1 un_a1 a2 a3 : val) (s_def s_pred : string)
-         K tᵥ (id : nat) m d ps pn B mlg,
+         K tᵥ (id : nat) m d ps pn ctr gm mlg,
       spec_verifier tᵥ (fill K (v_deser #id))
       ={⊤}=∗ ∃ (v_deser_par : val),
         spec_verifier tᵥ (fill K v_deser_par) ∗
         {{{ ⌜unsusp t' a1 un_a1⌝ ∗
             ▷ (lrel_tern_as_lrel A) a1 a2 a3 ∗
             susp_ser_p t' a1 s_def ∗
-            visited_mapg_auth m d ps pn B ∗
+            visited_mapg_auth m d ps pn ctr gm ∗
             lg_mapg_auth mlg ∗
             spec_verifier tᵥ (fill K (v_deser_par #s_pred)) }}}
           suspend un_a1
@@ -445,10 +445,10 @@ Section authenticatable_definitions.
                 ⌜p_sub_obj t a1' #lb⌝ ∗ ⌜v_sub_obj t a2' #susp⌝) ∗
               sub_susp_count t a2' c id c a2' ∗
               ser_v_proph t id a2' s_def ∗
-              visited_map_update_pending m d ps pn γl B) ∨
+              visited_map_update_pending m d ps pn γl ctr gm) ∨
             (⌜s_pred ≠ s_real⌝ ∗
               (lrel_tern_bin A) a1' a3 ∗
-              visited_mapg_auth m d ps pn B ∗
+              visited_mapg_auth m d ps pn ctr gm ∗
               ([∗ set] γ ∈ γl, ∃ lb,
                   visit_pending γ ∗ lg_mapg_frag lb γ ∗
                   ⌜p_sub_obj t a1' #lb⌝))) }}}).
